{
    "@context": {
        "as": "http://www.w3.org/ns/activitystreams#",
        "rdfs": "http://www.w3.org/2000/01/rdf-schema#",
        "type": "@type"
    },
    "@graph": [
        {
            "type": "rdfs:Class",
            "rdfs:comment": "Represent a unit of work",
            "rdfs:label": "Task",
            "rdfs:subClassOf": "as:Object"
        },
        {
            "type": "rdfs:Class",
            "rdfs:comment": "Represent a habit",
            "rdfs:label": "Habit",
            "rdfs:subClassOf": "as:Object"
        },
        {
            "type": "rdfs:Class",
            "rdfs:comment": "Represent an event of tracking a habit",
            "rdfs:label": "HabitTrackEvent",
            "rdfs:subClassOf": "as:Object"
        },
        {
            "type": "rdfs:Class",
            "rdfs:comment": "Indicates that an actor completed an object at the time of publishing this event",
            "rdfs:label": "Complete",
            "rdfs:subClassOf": "as:Activity"
        },
        {
            "type": "rdfs:Class",
            "rdfs:comment": "Indicates that an actor scheduled an object on a specific target",
            "rdfs:label": "Schedule",
            "rdfs:subClassOf": "as:Activity"
        },
        {
            "type": "rdfs:Class",
            "rdfs:comment": "Indicates that an actor started an object at the time of publishing this event",
            "rdfs:label": "Start",
            "rdfs:subClassOf": "as:Activity"
        },
        {
            "type": "rdfs:Class",
            "rdfs:comment": "Indicates that an actor finished an object at the time of publishing this event",
            "rdfs:label": "Finish",
            "rdfs:subClassOf": "as:Activity"
        },
        {
            "type": "rdfs:Property",
            "rdfs:comment": "A single emoji character representing an icon",
            "rdfs:label": "emojiIcon",
            "rdfs:range": "xsd:string"
        }
    ]
}
